requests.dfy
@@ -1,17 +1,29 @@
 import B = BloodRep
 
-method Matching(request: B.BloodType, inventory: array<B.BloodRecord>) returns (br: B.BloodRecord)
-{ 
-  
-}
-
-method Retrieve(br: B.BloodRecord, inventory: array<B.BloodRecord>) returns (success: bool) 
+// Assume inventory blood is sorted by expiry date
+// Gets an instance of the blood by the type
+method searchByType(bt: B.BloodType, inventory: array<B.BloodRecord>) returns (result: B.BloodRecord) 
 modifies inventory
+requires inventory != null
+requires !forall elm :: 0 <= elm < inventory.Length ==> inventory[elm].bType != bt
+requires exists elm :: 0 <= elm < inventory.Length && inventory[elm].bType == bt
 {
-
+  var i := 0;
+  while (i<inventory.Length) 
+  invariant 0 <= i <= inventory.Length
+  // Everything before the point being searched does not contain the correct type
+  invariant forall m :: 0 <= m < i ==> !sameType(inventory[m].bType, bt) 
+  {
+    if(inventory[i].bType == bt) {
+      result := inventory[i];
+      break;
+    }
+    assert (inventory[i].bType != bt);
+    i := i + 1; 
+  }
 }
 
-method Request(request: B.BloodType, inventory: array<B.BloodRecord>) returns (success: bool)
+function sameType(t1: B.BloodType, t2: B.BloodType): bool
 {
-
+  t1 == t2
 }
